Test/dafny0/RangeCompilation.dfy
@@ -1,4 +1,4 @@
-// RUN: %dafny /compile:3 "%s" > "%t"
+// RUN: %dafny /compile:3 /spillTargetCode:1 "%s" > "%t"
 // RUN: %diff "%s.expect" "%t"
 
 newtype Byte = x | 0 <= x < 256
@@ -9,6 +9,14 @@ predicate method GoodInteger(i: int) {
   i % 5 == 4
 }
 
+predicate method GoodChar(c: char) {
+  'a' <= c <= 'z'
+}
+
+predicate method GoodString(s: string) {
+    |s| > 0 && s[0] == 'x'
+}
+
 method Main() {
   assert GoodByte(11) && GoodInteger(24);
   var b: Byte :| GoodByte(b);
@@ -16,6 +24,14 @@ method Main() {
   print "b=", b, "  i=", i, "\n";
   var m0 := new MyClass;
   var m17 := new M17.AnotherClass;
+
+  var b2: bool :| b2;
+  assert GoodChar('q');
+  var c: char :| GoodChar(c);
+  var z: int :| z > 100;
+  assert GoodString("xylophone");
+  var my_strings: seq<string> := ["hello", "xylophone", "abc"];
+  var s: string :| s in my_strings && GoodString(s);
 }
 
 class MyClass { }
